memory_safety/classes.v
@@ -1,3 +1,4 @@
+Require Import ssreflect ssrfun ssrbool eqtype ssrnat.
 Require Import common.
 
 Set Implicit Arguments.
